verified/exceptions.i.dfy
@@ -1,0 +1,63 @@
+include "kom_common.i.dfy"
+include "entry.i.dfy"
+
+function {:opaque} dummyPageDb(): PageDb { imap[] }
+function {:opaque} dummyPageNr(): PageNr { 0 }
+
+predicate KomInterruptHandlerInvariant(s:state, sd:PageDb, r:state, dispPg:PageNr)
+    requires ValidState(s) && mode_of_state(s) != User && SaneMem(s.m)
+    requires s.conf.ex == ExFIQ || s.conf.ex == ExIRQ
+    requires priv_of_mode(spsr_of_state(s).m) == PL0 ==> (
+        validPageDb(sd) && pageDbCorresponds(s.m, sd)
+        && nonStoppedDispatcher(sd, dispPg))
+{
+    ValidState(r) && (s.ok ==> r.ok)
+    && SaneMem(r.m)
+    && SaneStack(r)
+    && ParentStackPreserving(s, r)
+    && GlobalsPreservingExcept(s, r, {PendingInterruptOp()})
+    && s.conf.ttbr0 == r.conf.ttbr0 && s.conf.scr == r.conf.scr
+    && if priv_of_mode(spsr_of_state(s).m) == PL1 then (
+        // if interrupted in privileged mode, we just set the pending flag
+        mode_of_state(r) == mode_of_state(s)
+        && spsr_of_state(r) == spsr_of_state(s)
+        && CoreRegPreservingExcept(s, r, {})
+        && BankedRegsInvariant(s, r)
+        && NonStackMemPreserving(s, r)
+    ) else (
+        mode_of_state(s) != User
+        && KomExceptionHandlerInvariant(s, sd, r, dispPg)
+    )
+}
+
+// this lemma is trivial, but justifies the soundness of the ARMdef assumptions
+// ("EssentialContinuationInvariantProperties") about the handler
+lemma lemma_KomInterruptHandlerInvariant_soundness(s:state, r:state)
+    requires ValidState(s) && mode_of_state(s) != User && SaneMem(s.m)
+    requires s.conf.ex == ExFIQ || s.conf.ex == ExIRQ
+    requires priv_of_mode(spsr_of_state(s).m) == PL1
+    requires KomInterruptHandlerInvariant(s, dummyPageDb(), r, dummyPageNr())
+    ensures EssentialContinuationInvariantProperties(s, r)
+{}
+
+predicate {:opaque} InterruptContinuationInvariantDef()
+{
+    reveal_ValidRegState();
+    forall s:state, r:state
+        | ValidState(s) && mode_of_state(s) != User && SaneMem(s.m)
+          && (s.conf.ex == ExFIQ || s.conf.ex == ExIRQ)
+          && priv_of_mode(spsr_of_state(s).m) == PL1
+        :: InterruptContinuationInvariant(s, r)
+        ==> KomInterruptHandlerInvariant(s, dummyPageDb(), r, dummyPageNr())
+}
+
+lemma lemma_InterruptContinuationInvariantDef(s:state, r:state)
+    requires InterruptContinuationInvariantDef()
+    requires ValidState(s) && mode_of_state(s) != User && SaneMem(s.m)
+    requires s.conf.ex == ExFIQ || s.conf.ex == ExIRQ
+    requires priv_of_mode(spsr_of_state(s).m) == PL1
+    requires InterruptContinuationInvariant(s, r)
+    ensures KomInterruptHandlerInvariant(s, dummyPageDb(), r, dummyPageNr())
+{
+    reveal_InterruptContinuationInvariantDef();
+}
